\section{TRIG \;IDENTITIES}
\subsubsection{Reciprocal Identities}

\begin{tabular}{m{5.5cm} m{5.5cm} m}
   $\sin \theta=\frac{1}{\csc \theta}$ & $\cos \theta=\frac{1}{\sec \theta}$ & $\tan \theta=\frac{1}{\cot \theta}$ \\
   $\csc \theta=\frac{1}{\sin \theta}$ & $\sec \theta=\frac{1}{\cos \theta}$ & $\cot \theta=\frac{1}{\tan \theta}$
\end{tabular}

\subsubsection{Quotient Identities}

\begin{tabular}{m{7cm} m}
    $\tan \theta=\frac{\sin \theta}{\cos \theta}$ & $\cot \theta=\frac{\cos \theta}{\sin \theta}$
\end{tabular}

\subsubsection{Pythagorean Identities}
\begin{tabular}{m{5.5cm} m{5.5cm} m}
    $1=\sin ^2 \theta+\cos ^2 \theta$ & $\sec ^2 \theta=\tan ^2 \theta+1$ & $\csc ^2 \theta=1+\cot ^2 \theta$ \\
\end{tabular}

\subsubsection{Even/Odd Identities}

\begin{tabular}{m{5cm} m{5cm} m}
    $\sin (-\theta)=-\sin \theta$ & $\cos (-\theta)=\cos \theta$ & $\tan (-\theta)=-\tan \theta$\\
    $\csc (-\theta)=-\csc \theta$ & $\sec (-\theta)=\sec \theta$ & $\cot (-\theta)=-\cot \theta$
\end{tabular}

\subsubsection{Cofunction Identities}

\begin{tabular}{m{5.5cm} m{5.5cm} m}
   $\sin \left(\frac{\pi}{2}-\theta\right)=\cos \theta$ & $\cos \left(\frac{\pi}{2}-\theta\right)=\sin \theta$ & $\tan \left(\frac{\pi}{2}-\theta\right)=\cot \theta$ \\
   $\csc \left(\frac{\pi}{2}-\theta\right)=\sec \theta$ & $\sec \left(\frac{\pi}{2}-\theta\right)=\csc \theta$ & $\cot \left(\frac{\pi}{2}-\theta\right)=\tan \theta$
\end{tabular}

\subsubsection{Sum and Difference Formulae} \label{SDF}

\begin{tabular}{m{7cm} m}
    $\sin (\alpha+\beta)=\sin \alpha \cos \beta+\sin \beta \cos \alpha$ & $\sin (\alpha-\beta)=\sin \alpha \cos \beta-\sin \beta \cos \alpha$ \\
    $\cos (\alpha+\beta)=\cos \alpha \cos \beta-\sin \alpha \sin \beta$ & $\cos (\alpha-\beta)=\cos \alpha \cos \beta+\sin \alpha \sin \beta$\\
    $\tan (\alpha+\beta)=\frac{\tan \alpha+\tan \beta}{1-\tan \alpha \tan \beta}$ & $\tan(\alpha-\beta)=\frac{\tan \alpha-\tan \beta}{1+\tan \alpha \tan \beta}$
\end{tabular}

\textbf{Note:} The following three kinds of identities can all be derived from the Sum and Difference Formulae.

\subsubsection{Double Angle Identities}

\begin{tabular}{m{5.5cm} m{5.5cm} m}
    $\sin 2 \theta=2 \sin \theta \cos \theta$ & $\tan 2 \theta=\frac{2 \tan \theta}{1-\tan ^2 \theta}$ & $\cos 2 \theta =1-2 \sin ^2 \theta$ \\
\end{tabular}

\subsubsection{Power Reducing Identities}

\begin{tabular}{m{5.5cm} m{5.5cm} m}
    $\sin ^2 \theta=\frac{1-\cos 2 \theta}{2}$ & $\cos ^2 \theta=\frac{1+\cos 2 \theta}{2}$ & $\tan ^2 \theta=\frac{1-\cos 2 \theta}{1+\cos 2 \theta}$ \\
\end{tabular}

\subsubsection{Half Angle Identities}

\begin{tabular}{m{5.5cm} m{5.5cm} m}
    $\sin \frac{\theta}{2}=\pm \sqrt{\frac{1-\cos \theta}{2}}$ & $\cos \frac{\theta}{2}=\pm \sqrt{\frac{1+\cos \theta}{2}}$ & $\tan \frac{\theta}{2}=\frac{1-\cos \theta}{\sin \theta}=\frac{\sin \theta}{1+\cos \theta}$ \\
\end{tabular}

\subsubsection{Product to Sum Identities}

\begin{tabular}{m{8cm} m}
    $\sin \alpha \sin \beta=\frac{1}{2}[\cos (\alpha-\beta)-\cos (\alpha+\beta)]$ & $\cos \alpha \cos \beta=\frac{1}{2}[\cos (\alpha-\beta)+\cos (\alpha+\beta)]$\\
    $\sin \alpha \cos \beta=\frac{1}{2}[\sin (\alpha-\beta)+\sin (\alpha+\beta)]$ &
\end{tabular}

\subsubsection{Sum to Product Identities}

\begin{tabular}{m{8cm} m}
    $\sin \alpha+\sin \beta=2 \sin \left(\frac{\alpha+\beta}{2}\right) \cos \left(\frac{\alpha-\beta}{2}\right)$ & $ \sin \alpha-\sin \beta=2 \cos \left(\frac{\alpha+\beta}{2}\right) \sin \left(\frac{\alpha-\beta}{2}\right)$\\
    $\cos \alpha+\cos \beta=2 \cos \left(\frac{\alpha+\beta}{2}\right) \cos \left(\frac{\alpha-\beta}{2}\right)$ & $\cos \alpha-\cos \beta=-2 \sin \left(\frac{\alpha+\beta}{2}\right) \sin \left(\frac{\alpha-\beta}{2}\right)$
\end{tabular}
